MemOps.v
@@ -18,6 +18,7 @@ Section memops.
       memOpName := Lb;
       memOpCode := 0;
       memOpSize := 0;
+      memOpAmoClass := None;
       memOpRegValue := memRegValueFn (fun _ mem => RetE (sign_extend_trunc 8 Rlen mem));
       memOpWriteValue := memWriteValueNone
     |};
@@ -25,6 +26,7 @@ Section memops.
       memOpName := Lh;
       memOpCode := 1;
       memOpSize := 1;
+      memOpAmoClass := None;
       memOpRegValue := memRegValueFn (fun _ mem => RetE (sign_extend_trunc 16 Rlen mem));
       memOpWriteValue := memWriteValueNone
     |};
@@ -32,6 +34,7 @@ Section memops.
       memOpName := Lw;
       memOpCode := 2;
       memOpSize := 2;
+      memOpAmoClass := None;
       memOpRegValue := memRegValueFn (fun _ mem => RetE (sign_extend_trunc 32 Rlen mem));
       memOpWriteValue := memWriteValueNone
     |};
@@ -39,6 +42,7 @@ Section memops.
       memOpName := Lbu;
       memOpCode := 3;
       memOpSize := 0;
+      memOpAmoClass := None;
       memOpRegValue := memRegValueFn (fun _ mem => RetE (zero_extend_trunc 8 Rlen mem));
       memOpWriteValue := memWriteValueNone
     |};
@@ -46,6 +50,7 @@ Section memops.
       memOpName := Lhu;
       memOpCode := 4;
       memOpSize := 1;
+      memOpAmoClass := None;
       memOpRegValue := memRegValueFn (fun _ mem => RetE (zero_extend_trunc 16 Rlen mem));
       memOpWriteValue := memWriteValueNone
     |};
@@ -53,6 +58,7 @@ Section memops.
       memOpName := Lwu;
       memOpCode := 5;
       memOpSize := 2;
+      memOpAmoClass := None;
       memOpRegValue := memRegValueFn (fun _ mem => RetE (zero_extend_trunc 32 Rlen mem));
       memOpWriteValue := memWriteValueNone
     |};
@@ -60,6 +66,7 @@ Section memops.
       memOpName := Ld;
       memOpCode := 6;
       memOpSize := 3;
+      memOpAmoClass := None;
       memOpRegValue := memRegValueFn (fun _ mem => RetE mem);
       memOpWriteValue := memWriteValueNone
     |};
@@ -67,6 +74,7 @@ Section memops.
       memOpName := Sb;
       memOpCode := 7;
       memOpSize := 0;
+      memOpAmoClass := None;
       memOpRegValue := memRegValueNone;
       memOpWriteValue := memWriteValueStore
     |};
@@ -74,6 +82,7 @@ Section memops.
       memOpName := Sh;
       memOpCode := 8;
       memOpSize := 1;
+      memOpAmoClass := None;
       memOpRegValue := memRegValueNone;
       memOpWriteValue := memWriteValueStore
     |};
@@ -81,6 +90,7 @@ Section memops.
       memOpName := Sw;
       memOpCode := 9;
       memOpSize := 2;
+      memOpAmoClass := None;
       memOpRegValue := memRegValueNone;
       memOpWriteValue := memWriteValueStore
     |};
@@ -88,6 +98,7 @@ Section memops.
       memOpName := Sd;
       memOpCode := 10;
       memOpSize := 3;
+      memOpAmoClass := None;
       memOpRegValue := memRegValueNone;
       memOpWriteValue := memWriteValueStore
     |};
@@ -95,6 +106,7 @@ Section memops.
       memOpName := Flw;
       memOpCode := 11;
       memOpSize := 2;
+      memOpAmoClass := None;
       memOpRegValue := memRegValueFn (fun _ mem => RetE (one_extend_trunc 32 Rlen mem));
       memOpWriteValue := memWriteValueNone
     |};
@@ -102,6 +114,7 @@ Section memops.
       memOpName := Fld;
       memOpCode := 12;
       memOpSize := 3;
+      memOpAmoClass := None;
       memOpRegValue := memRegValueFn (fun _ mem => RetE mem);
       memOpWriteValue := memWriteValueNone
     |};
@@ -109,6 +122,7 @@ Section memops.
       memOpName := Fsw;
       memOpCode := 13;
       memOpSize := 2;
+      memOpAmoClass := None;
       memOpRegValue := memRegValueNone;
       memOpWriteValue := memWriteValueStore
     |};
@@ -116,6 +130,7 @@ Section memops.
       memOpName := Fsd;
       memOpCode := 14;
       memOpSize := 3;
+      memOpAmoClass := None;
       memOpRegValue := memRegValueNone;
       memOpWriteValue := memWriteValueStore
     |};
@@ -123,6 +138,7 @@ Section memops.
       memOpName := AmoSwapW;
       memOpCode := 15;
       memOpSize := 2;
+      memOpAmoClass := Some AmoSwap;
       memOpRegValue := memRegValueFn (fun _ mem => RetE (sign_extend_trunc 32 Rlen mem));
       memOpWriteValue := memWriteValueFn (fun _ reg _ => RetE (SignExtendTruncLsb Rlen ((unsafeTruncLsb 32 reg))))
     |};
@@ -130,6 +146,7 @@ Section memops.
       memOpName := AmoAddW;
       memOpCode := 16;
       memOpSize := 2;
+      memOpAmoClass := Some AmoArith;
       memOpRegValue := memRegValueFn (fun _ mem => RetE (sign_extend_trunc 32 Rlen mem));
       memOpWriteValue := memWriteValueFn (fun _ reg mem => RetE (SignExtendTruncLsb Rlen ((unsafeTruncLsb 32 reg) + (unsafeTruncLsb 32 mem))))
     |};
@@ -137,6 +154,7 @@ Section memops.
       memOpName := AmoXorW;
       memOpCode := 17;
       memOpSize := 2;
+      memOpAmoClass := Some AmoLogical;
       memOpRegValue := memRegValueFn (fun _ mem => RetE (sign_extend_trunc 32 Rlen mem));
       memOpWriteValue := memWriteValueFn (fun _ reg mem => RetE (SignExtendTruncLsb Rlen ((unsafeTruncLsb 32 reg) .^ (unsafeTruncLsb 32 mem))))
     |};
@@ -144,6 +162,7 @@ Section memops.
       memOpName := AmoAndW;
       memOpCode := 18;
       memOpSize := 2;
+      memOpAmoClass := Some AmoLogical;
       memOpRegValue := memRegValueFn (fun _ mem => RetE (sign_extend_trunc 32 Rlen mem));
       memOpWriteValue := memWriteValueFn (fun _ reg mem => RetE (SignExtendTruncLsb Rlen ((unsafeTruncLsb 32 reg) .&  (unsafeTruncLsb 32 mem))))
     |};
@@ -151,6 +170,7 @@ Section memops.
       memOpName := AmoOrW;
       memOpCode := 19;
       memOpSize := 2;
+      memOpAmoClass := Some AmoLogical;
       memOpRegValue := memRegValueFn (fun _ mem => RetE (sign_extend_trunc 32 Rlen mem));
       memOpWriteValue := memWriteValueFn (fun _ reg mem => RetE (SignExtendTruncLsb Rlen ((unsafeTruncLsb 32 reg) .| (unsafeTruncLsb 32 mem))))
     |};
@@ -158,6 +178,7 @@ Section memops.
       memOpName := AmoMinW;
       memOpCode := 20;
       memOpSize := 2;
+      memOpAmoClass := Some AmoArith;
       memOpRegValue := memRegValueFn (fun _ mem => RetE (sign_extend_trunc 32 Rlen mem));
       memOpWriteValue := memWriteValueFn (fun _ reg mem => RetE (IF (SignExtendTruncLsb 32 reg) >s (SignExtendTruncLsb (31+1) mem) then mem else reg))
     |};
@@ -165,6 +186,7 @@ Section memops.
       memOpName := AmoMaxW;
       memOpCode := 21;
       memOpSize := 2;
+      memOpAmoClass := Some AmoArith;
       memOpRegValue := memRegValueFn (fun _ mem => RetE (sign_extend_trunc 32 Rlen mem));
       memOpWriteValue := memWriteValueFn (fun _ reg mem => RetE (IF (SignExtendTruncLsb 32 reg) >s (SignExtendTruncLsb (31+1) mem) then reg else mem))
     |};
@@ -172,6 +194,7 @@ Section memops.
       memOpName := AmoMinuW;
       memOpCode := 22;
       memOpSize := 2;
+      memOpAmoClass := Some AmoArith;
       memOpRegValue := memRegValueFn (fun _ mem => RetE (sign_extend_trunc 32 Rlen mem));
       memOpWriteValue := memWriteValueFn (fun _ reg mem => RetE (IF (ZeroExtendTruncLsb 32 reg) > (ZeroExtendTruncLsb 32 mem) then mem else reg))
     |};
@@ -179,6 +202,7 @@ Section memops.
       memOpName := AmoMaxuW;
       memOpCode := 23;
       memOpSize := 2;
+      memOpAmoClass := Some AmoArith;
       memOpRegValue := memRegValueFn (fun _ mem => RetE (sign_extend_trunc 32 Rlen mem));
       memOpWriteValue := memWriteValueFn (fun _ reg mem => RetE (IF reg > mem then reg else mem))
     |};
@@ -186,6 +210,7 @@ Section memops.
       memOpName := AmoSwapD;
       memOpCode := 24;
       memOpSize := 3;
+      memOpAmoClass := Some AmoSwap;
       memOpRegValue := memRegValueFn (fun _ mem => RetE mem);
       memOpWriteValue := memWriteValueFn (fun _ reg _ => RetE reg)
     |};
@@ -193,6 +218,7 @@ Section memops.
       memOpName := AmoAddD;
       memOpCode := 25;
       memOpSize := 3;
+      memOpAmoClass := Some AmoArith;
       memOpRegValue := memRegValueFn (fun _ mem => RetE mem);
       memOpWriteValue := memWriteValueFn (fun _ reg mem => RetE (reg + mem))
     |};
@@ -200,6 +226,7 @@ Section memops.
       memOpName := AmoXorD;
       memOpCode := 26;
       memOpSize := 3;
+      memOpAmoClass := Some AmoLogical;
       memOpRegValue := memRegValueFn (fun _ mem => RetE mem);
       memOpWriteValue := memWriteValueFn (fun _ reg mem => RetE (reg .^ mem))
     |};
@@ -207,6 +234,7 @@ Section memops.
       memOpName := AmoAndD;
       memOpCode := 27;
       memOpSize := 3;
+      memOpAmoClass := Some AmoLogical;
       memOpRegValue := memRegValueFn (fun _ mem => RetE mem);
       memOpWriteValue := memWriteValueFn (fun _ reg mem => RetE (reg .&  mem))
     |};
@@ -214,6 +242,7 @@ Section memops.
       memOpName := AmoOrD;
       memOpCode := 28;
       memOpSize := 3;
+      memOpAmoClass := Some AmoLogical;
       memOpRegValue := memRegValueFn (fun _ mem => RetE mem);
       memOpWriteValue := memWriteValueFn (fun _ reg mem => RetE (reg .| mem))
     |};
@@ -221,6 +250,7 @@ Section memops.
       memOpName := AmoMinD;
       memOpCode := 29;
       memOpSize := 3;
+      memOpAmoClass := Some AmoArith;
       memOpRegValue := memRegValueFn (fun _ mem => RetE mem);
       memOpWriteValue := memWriteValueFn (fun _ reg mem => RetE (IF (SignExtendTruncLsb 64 reg) >s (SignExtendTruncLsb (63+1) mem) then mem else reg))
     |};
@@ -228,6 +258,7 @@ Section memops.
       memOpName := AmoMaxD;
       memOpCode := 30;
       memOpSize := 3;
+      memOpAmoClass := Some AmoArith;
       memOpRegValue := memRegValueFn (fun _ mem => RetE mem);
       memOpWriteValue := memWriteValueFn (fun _ reg mem => RetE (IF (SignExtendTruncLsb 64 reg) >s (SignExtendTruncLsb (63+1) mem) then reg else mem))
     |};
@@ -235,6 +266,7 @@ Section memops.
       memOpName := AmoMinuD;
       memOpCode := 31;
       memOpSize := 3;
+      memOpAmoClass := Some AmoArith;
       memOpRegValue := memRegValueFn (fun _ mem => RetE mem);
       memOpWriteValue := memWriteValueFn (fun _ reg mem => RetE (IF (ZeroExtendTruncLsb 64 reg) > (ZeroExtendTruncLsb 64 mem) then mem else reg))
     |};
@@ -242,6 +274,7 @@ Section memops.
       memOpName := AmoMaxuD;
       memOpCode := 32;
       memOpSize := 3;
+      memOpAmoClass := Some AmoArith;
       memOpRegValue := memRegValueFn (fun _ mem => RetE mem);
       memOpWriteValue := memWriteValueFn (fun _ reg mem => RetE (IF reg > mem then reg else mem))
     |};
@@ -249,6 +282,7 @@ Section memops.
       memOpName := LrW;
       memOpCode := 33;
       memOpSize := 2;
+      memOpAmoClass := None;
       memOpRegValue := memRegValueFn (fun _ mem => RetE (sign_extend_trunc 32 Rlen mem));
       memOpWriteValue := memWriteValueNone
     |};
@@ -256,6 +290,7 @@ Section memops.
       memOpName := ScW;
       memOpCode := 34;
       memOpSize := 2;
+      memOpAmoClass := None;
       memOpRegValue := memRegValueNone;
       memOpWriteValue := memWriteValueStore
     |};
@@ -263,6 +298,7 @@ Section memops.
       memOpName := LrD;
       memOpCode := 35;
       memOpSize := 3;
+      memOpAmoClass := None;
       memOpRegValue := memRegValueFn (fun _ mem => RetE (sign_extend_trunc 64 Rlen mem));
       memOpWriteValue := memWriteValueNone
     |};
@@ -270,6 +306,7 @@ Section memops.
       memOpName := ScD;
       memOpCode := 36;
       memOpSize := 3;
+      memOpAmoClass := None;
       memOpRegValue := memRegValueNone;
       memOpWriteValue := memWriteValueStore
     |}
